State monotonicity theorem with state assumptions
... and incorporate proofs of state invariant preservation.

CHERI_Monotonicity.thy
@@ -5,6 +5,7 @@ theory CHERI_Monotonicity
     CHERI_Cap_Properties
     CHERI_Mem_Properties
     CHERI_Fetch_Properties
+    Morello_Invariants
     "Sail-T-CHERI.Trace_Assumptions"
     "Sail-T-CHERI.Properties"
 begin
@@ -88,21 +89,37 @@ locale Morello_Fetch_Trace_Mem_Automaton =
 context Morello_Fixed_Address_Translation
 begin
 
-abbreviation "instr_assms instr t \<equiv> Morello_Instr_Trace_Write_Cap_Automaton.instr_trace_assms translate_address is_translation_event translation_assms UNKNOWN_caps t"
-abbreviation "fetch_assms t \<equiv> Morello_Fetch_Trace_Write_Cap_Automaton.fetch_trace_assms translate_address is_translation_event translation_assms UNKNOWN_caps t"
+abbreviation "s_read_from reg s \<equiv> read_from reg (regstate s)"
 
-(* TODO:
-   - Restrict ex_traces case to only exceptions, not failures; clean up instr/fetch_raises_ex again
- *)
+abbreviation "pcc_not_sealed s \<equiv> (let pcc = s_read_from PCC_ref s in CapIsTagSet pcc \<longrightarrow> \<not>CapIsSealed pcc)"
+abbreviation "pcc_tagged s \<equiv> CapIsTagSet (s_read_from PCC_ref s)"
+abbreviation "non_debug_state s \<equiv> ((ucast (s_read_from EDSCR_ref s) :: 6 word) = 2)"
+abbreviation "cache_line_size_64 s \<equiv> ((ucast (s_read_from DCZID_EL0_ref s) :: 4 word) = 4)"
 
-sublocale CHERI_ISA CC ISA cap_invariant UNKNOWN_caps fetch_assms instr_assms
+definition "fetch_state_assms s \<equiv> pcc_not_sealed s \<and> non_debug_state s \<and> cache_line_size_64 s"
+definition "instr_state_assms _ s \<equiv> fetch_state_assms s \<and> pcc_tagged s"
+
+text \<open>TODO: Show that the trace assumptions (apart from the translation and UNKNOWN cap ones) are
+  implied by the state assumptions and reduce the following to the remaining trace assumptions.\<close>
+abbreviation "instr_trace_assms instr t \<equiv> Morello_Instr_Trace_Write_Cap_Automaton.instr_trace_assms translate_address is_translation_event translation_assms UNKNOWN_caps t"
+abbreviation "fetch_trace_assms t \<equiv> Morello_Fetch_Trace_Write_Cap_Automaton.fetch_trace_assms translate_address is_translation_event translation_assms UNKNOWN_caps t"
+
+abbreviation "s_translate_address addr acctype s \<equiv> translate_address addr"
+
+interpretation Register_State get_regval set_regval
+  apply standard
+  sorry
+
+interpretation Morello_Register_Accessors ..
+
+sublocale CHERI_ISA_State CC ISA cap_invariant UNKNOWN_caps fetch_trace_assms fetch_state_assms instr_trace_assms instr_state_assms get_regval set_regval s_translate_address
 proof
   fix t :: "register_value trace" and instr :: instr and n :: nat
   interpret Write_Cap: Morello_Instr_Trace_Write_Cap_Automaton where instr = instr and t = t
     by standard (auto simp: trace_uses_mem_caps_def)
   assume t: "hasTrace t (instr_sem_ISA instr)"
     and inv: "instr_available_caps_invariant instr t n"
-    and ia: "instr_assms instr t"
+    and ia: "instr_trace_assms instr t"
     and n: "n \<le> length t"
   from t have iea: "Write_Cap.instr_exp_assms (instr_sem instr)"
     by (intro Write_Cap.instr_exp_assms_instr_semI) simp
@@ -130,7 +147,7 @@ next
     by standard auto
   assume t: "hasTrace t (isa.instr_fetch ISA)"
     and inv: "fetch_available_caps_invariant t n"
-    and ia: "fetch_assms t"
+    and ia: "fetch_trace_assms t"
     and n: "n \<le> length t"
   from ia have no_asr: "\<not>trace_has_system_reg_access t"
     by simp
@@ -149,18 +166,78 @@ next
     by (intro conjI; elim Write_Cap.traces_enabled_reg_axioms Mem.traces_enabled_mem_axioms)
        (auto simp: fetch_raises_ex_def Write_Cap.trace_raises_isa_exception_def
              elim: is_isa_exception.elims intro: Write_Cap.holds_along_trace_take)
-qed
+qed auto
 
-abbreviation "s_translate_address addr acctype s \<equiv> translate_address addr"
+abbreviation "unknown_caps_of_trace t \<equiv> {c. E_choose ''UNKNOWN_Capability'' (Regval_bitvector_129_dec c) \<in> set t}"
+abbreviation "unknown_caps_reachable t s \<equiv> unknown_caps_of_trace t \<subseteq> UNKNOWN_caps \<and> UNKNOWN_caps \<subseteq> reachable_caps s"
 
-interpretation Morello_Register_State: Register_State get_regval set_regval
-  apply standard
-  sorry
+lemma fetch_state_assms_iff_invs:
+  "fetch_state_assms s \<longleftrightarrow> PCC_inv s \<and> EDSCR_inv s \<and> DCZID_inv s"
+  unfolding fetch_state_assms_def EDSCR_inv_def DCZID_inv_def reg_inv_def Let_def
+  by (auto simp: register_defs regval_of_bitvector_129_dec_def regval_of_bitvector_32_dec_def)
 
-sublocale CHERI_ISA_State CC ISA cap_invariant UNKNOWN_caps fetch_assms instr_assms get_regval set_regval s_translate_address
-  by standard auto
-
-thm reachable_caps_instrs_trace_intradomain_monotonicity
+lemma
+  assumes "hasTrace t (fetch_execute_loop ISA n)"
+    and "s_run_trace t s = Some s'"
+    and "\<forall>c\<in>reachable_caps s. is_tagged_method CC c \<longrightarrow> cap_invariant c"
+    and "\<not>instrs_raise_ex ISA n t"
+    and "instrs_invoke_caps ISA n t \<union> instrs_invoke_indirect_caps ISA n t \<subseteq> reachable_caps s"
+    and "\<not>system_access_reachable s"
+    and "translation_assms_trace t"
+    and "unknown_caps_reachable t s"
+    and "pcc_not_sealed s"
+    and "non_debug_state s"
+    and "cache_line_size_64 s"
+    and "instrs_trace_assms n t" \<comment> \<open>TODO: Show that the above assumptions imply this\<close>
+  shows "reachable_caps s' \<subseteq> reachable_caps s"
+proof (rule reachable_caps_instrs_trace_intradomain_monotonicity[OF assms(1)])
+  show "instrs_preserve_state_assms s"
+  proof (unfold instrs_preserve_state_assms_plus_def, intro allI impI, elim conjE)
+    fix ti instr si si'
+    assume ti: "Run (instr_sem_ISA instr) ti ()" "s_run_trace ti si = Some si'"
+      and si: "instr_state_assms instr si"
+    have "runs_preserve_invariant (liftS (instr_sem instr)) fetch_state_assms"
+      unfolding fetch_state_assms_iff_invs
+      by (intro runs_preserve_invariant_conjI instr_sem_preserves_PCC_inv instr_sem_preserves_EDSCR_inv instr_sem_preserves_DCZID_inv)
+    then show "fetch_state_assms si'"
+      using Run_runTraceS_Value_liftState[OF ti] si
+      by (auto simp: instr_state_assms_def elim: PrePostE_elim)
+  qed
+  show "fetch_preserves_state_assms s"
+  proof (unfold fetch_preserves_state_assms_plus_def, intro allI impI, elim conjE)
+    fix tf instr sf sf'
+    assume tf: "Run (isa.instr_fetch ISA) tf instr" "s_run_trace tf sf = Some sf'"
+      and sf: "fetch_state_assms sf"
+    have "runs_preserve_invariant (liftS instr_fetch) fetch_state_assms"
+      unfolding fetch_state_assms_iff_invs
+      by (intro runs_preserve_invariant_conjI instr_fetch_preserves_PCC_inv instr_fetch_preserves_EDSCR_inv instr_fetch_preserves_DCZID_inv)
+    moreover have "runs_establish_invariant (liftS instr_fetch) pcc_tagged"
+    proof -
+      \<comment> \<open>TODO: Rephrase and move FetchInstr lemma out of its probably overspecific context, so that
+          we don't have to instantiate this locale here and translate the invariant back and forth.\<close>
+      interpret Write_Cap: Morello_Fetch_Trace_Write_Cap_Automaton where t = tf
+        by standard auto
+      let ?tagged_reg = "\<lambda>v. case v of Regval_bitvector_129_dec c \<Rightarrow> CapIsTagSet c | _ \<Rightarrow> True"
+      have FetchInstr: "runs_establish_invariant (liftS (FetchInstr pc)) (reg_inv ''PCC'' ?tagged_reg)" for pc
+        using Write_Cap.PrePostE_FetchInstr_pcc_tagged_unsealed[where pc = pc]
+        by (elim PrePostE_weaken_post) (auto simp: register_defs regval_of_bitvector_129_dec_def reg_inv_def)
+      have "runs_establish_invariant (liftS instr_fetch) (reg_inv ''PCC'' ?tagged_reg)"
+        unfolding instr_fetch_def FetchNextInstr_def liftState_simp comp_def
+        by (intro FetchInstr[THEN runs_establish_invariant_bindS_left] runs_establish_invariant_bindS_right)
+           (auto simp: no_reg_writes_runs_no_reg_writes)
+      then show ?thesis
+        by (elim PrePostE_weaken_post) (auto simp: register_defs regval_of_bitvector_129_dec_def reg_inv_def)
+    qed
+    ultimately show "instr_state_assms instr sf'"
+      using Run_runTraceS_Value_liftState[OF tf] sf
+      by (auto simp: instr_state_assms_def elim: PrePostE_elim)
+  qed
+  show "s_invariant_holds (addr_trans_invariant False s) t s"
+    \<comment> \<open>Holds trivially because of the Morello_Fixed_Address_Translation setup;  the real proof
+        obligations about the actual address translation will show up when instantiating that locale.\<close>
+    by (rule take_s_invariant_holdsI[OF \<open>s_run_trace t s = Some s'\<close>])
+       (auto simp: addr_trans_invariant_plus_def)
+qed (use assms in \<open>auto simp: fetch_state_assms_def\<close>)
 
 end
 
